starting to make progress

btree.dfy
@@ -46,6 +46,24 @@ lemma lexical_cmp_between_implies_common_prefix(a: string, b: string, c: string)
 	}
 }
 
+//////////////////////////////////////////////
+
+function method min(a: int, b: int) : int
+{
+	if a < b
+		then a
+	else
+		b
+}
+
+function method max(a: int, b: int) : int
+{
+	if a < b
+		then b
+	else
+		a
+}
+
 ///////////////////////////////////////////
 
 function method seq_map<U,T>(f: T-> U, inputs: seq<T>) : seq<U>
@@ -61,150 +79,69 @@ function method seq_fold_left<U,T>(f: (U, T) -> U, acc: U, inputs: seq<T>) : U
 	else seq_fold_left(f, f(acc, inputs[0]), inputs[1..])
 }
 
+function method seq_min(s: seq<int>) : int
+	requires |s| > 0;
+{
+	seq_fold_left((a, b) => min(a, b), s[0], s[1..])
+}
+
+function method seq_max(s: seq<int>) : int
+	requires |s| > 0;
+{
+	seq_fold_left((a, b) => max(a, b), s[0], s[1..])
+}
+
+function method seq_sum(s: seq<int>) : int
+	requires |s| > 0;
+{
+	seq_fold_left((a, b) => a + b, 0, s)
+}
+
+function method seq_union<T>(s: seq<set<T> >) : set<T>
+	requires |s| > 0;
+{
+	seq_fold_left((a, b) => a + b, {}, s)
+}
+
+////////////////////////////////////////////
+
 datatype Node =
 	Leaf(keys: seq<string>, values: seq<int>) |
 	Index(pivots: seq<string>, children: seq<Node>)
 
-// function num_nodes(node: Node) : int
-// {
-// 	match node {
-// 		case Leaf(keys, values) => 1
-// 		case Index(pivots, children) =>
-			
-// 	}
-// }
-
-function method set_of_keys_of_children(nodes: seq<Node>, ghost height: int, ghost max_fanout: int) : set<string>
-	decreases height * max_fanout;
-{
-	if |nodes| == 0 then {}
-	else set_of_keys(nodes[0], m-1) + set_of_keys_of_children(nodes[1..], m)
-}
-
-function method set_of_keys(node: Node, ghost m: int) : set<string>
-	requires m == num_nodes(node);
-	//requires subtree_is_well_formed(node);
-	//decreases node;
-	decreases m;
-{	
+predicate subtree_is_well_formed(node: Node) {
 	match node {
 		case Leaf(keys, values) =>
-			set k | k in multiset(keys)
+			|keys| > 0 &&
+			|keys| == |values|
 		case Index(pivots, children) =>
-			children_have_lower_max_height(node);
-			//seq_fold_left((a, b) => a + b, {}, seq_map(x => set_of_keys(x), children))
-			set_of_keys_of_children(children, m-1)
+			|pivots| > 0 &&
+			|pivots| == |children| - 1 &&
+			forall child :: child in children ==> subtree_is_well_formed(child)
 	}
 }
 
-// predicate subtree_is_well_formed(node: Node) {
-// 	match node {
-// 		case Leaf(keys, values) =>
-// 			|keys| > 0 &&
-// 			|keys| == |values|
-// 		case Index(pivots, children) =>
-// 			|pivots| > 0 &&
-// 			|pivots| == |children| - 1 &&
-// 			forall i :: 0 <= i < |children| ==> subtree_is_well_formed(children[i])
-// 	}
-// }
-
-// predicate seq_is_strictly_increasing(ss: seq<string>) {
-// 	forall i :: 0 <= i < |ss|-1 ==> lexical_cmp(ss[i], ss[i+1]) < 0
-// }		
-
-// predicate subtree_is_sorted(node: Node)
-// 	requires subtree_is_well_formed(node);
-// {
-// 	match node {
-// 		case Leaf(keys, values) =>
-// 			seq_is_strictly_increasing(keys)
-// 		case Index(pivots, children) =>
-// 			seq_is_strictly_increasing(pivots) &&
-// 			(forall i :: 0 <= i < |children|-1 ==>
-// 			  (forall x :: x in set_of_keys(children[i]) ==>
-// 			    lexical_cmp(x, pivots[i]) < 0)) &&
-// 			(forall i :: 1 <= i < |children| ==>
-// 			  (forall x :: x in set_of_keys(children[i]) ==>
-// 			    lexical_cmp(pivots[i-1], x) <= 0)) &&
-// 			forall i :: 0 <= i < |children| ==> subtree_is_sorted(children[i])
-// 	}
-// }
-
-// function map_of_kvpairs(acc: map<string, int>, keys: seq<string>, values: seq<int>) : map<string, int>
-// 	requires |keys| == |values|;
-// {
-// 	if |keys| == 0 then acc
-// 	else map_of_kvpairs(acc, keys[1..], values[1..])[keys[0] := values[0]]
-// }
-
-// function map_of_children(acc: map<string, int>, nodes: seq<Node>) : map<string, int>
-// 	requires forall i :: 0 <= i < |nodes| ==> subtree_is_well_formed(nodes[i]);
-// 	requires forall i :: 0 <= i < |nodes| ==> subtree_is_sorted(nodes[i]);
-// {
-// 	if |nodes| == 0 then acc
-// 	else map_of_children(map_of_subtree(acc, nodes[0]), nodes[1..])
-// }
-
-// function map_of_subtree(acc: map<string, int>, node: Node) : map<string, int>
-// 	requires subtree_is_well_formed(node);
-// 	requires subtree_is_sorted(node);
-// {
-// 	match node {
-// 		case Leaf(keys, values) =>
-// 			map_of_kvpairs(acc, keys, values)
-// 		case Index(pivots, children) =>
-// 			max_height_is_nonnegative(node);
-// 			assert forall i :: 0 <= i < |children| ==> max_height(children[i]) < max_height(node);
-// 			map_of_children(acc, children)
-// 	}
-// }
-
-// function subtree_map_contents(node: Node) : map<string, int>
-// 	requires subtree_is_well_formed(node);
-// 	requires subtree_is_sorted(node);
-// {
-// 	map_of_subtree(map[], node)
-// }
-
-// function method min(a: int, b: int) : int
-// {
-// 	if a < b
-// 		then a
-// 	else
-// 		b
-// }
-
-function method max(a: int, b: int) : int
+function min_height_of_children(nodes: seq<Node>) : int
+	requires forall i :: 0 <= i < |nodes| ==> subtree_is_well_formed(nodes[i]);
+	requires |nodes| > 0;
 {
-	if a < b
-		then b
-	else
-		a
+	if |nodes| == 1 then min_height(nodes[0])
+	else min(min_height(nodes[0]), min_height_of_children(nodes[1..]))
 }
 
-// function min_height_of_children(nodes: seq<Node>) : int
-// 	requires forall i :: 0 <= i < |nodes| ==> subtree_is_well_formed(nodes[i]);
-// 	requires |nodes| > 0;
-// {
-// 	if |nodes| == 1 then min_height(nodes[0])
-// 	else min(min_height(nodes[0]), min_height_of_children(nodes[1..]))
-// }
-
-// function min_height(node: Node) : int
-// 	requires subtree_is_well_formed(node);
-// {
-// 	match node {
-// 		case Leaf(keys, values) => 0
-// 		case Index(pivots, children) => 1 + min_height_of_children(children)
-// 	}
-// }
+function min_height(node: Node) : int
+	requires subtree_is_well_formed(node);
+{
+	match node {
+		case Leaf(keys, values) => 0
+		case Index(pivots, children) =>
+			1 + min_height_of_children(children)
+	}
+}
 
 function max_height_of_children(nodes: seq<Node>) : int
-	//requires forall i :: 0 <= i < |nodes| ==> subtree_is_well_formed(nodes[i]);
-	//requires |nodes| > 0;
-	ensures max_height_of_children(nodes) >= 0;
-	ensures forall i :: 0 <= i < |nodes| ==> max_height(nodes[i]) <= max_height_of_children(nodes);
+	requires forall i :: 0 <= i < |nodes| ==> subtree_is_well_formed(nodes[i]);
+	requires |nodes| > 0;
 {
 	if |nodes| == 0 then 0
 	else if |nodes| == 1 then max_height(nodes[0])
@@ -212,87 +149,186 @@ function max_height_of_children(nodes: seq<Node>) : int
 }
 
 function max_height(node: Node) : int
-	//requires subtree_is_well_formed(node);
+	requires subtree_is_well_formed(node);
 	ensures max_height(node) >= 0;
 {
 	match node {
 		case Leaf(keys, values) => 0
-		case Index(pivots, children) => 1 + max_height_of_children(children)
+		case Index(pivots, children) =>
+			1 + max_height_of_children(children)
 	}
 }
 
-lemma max_height_is_nonnegative(node: Node)
-	//requires subtree_is_well_formed(node);
-	ensures max_height(node) >= 0;
+predicate subtree_is_balanced(node: Node)
+	requires subtree_is_well_formed(node);
 {
+	min_height(node) == max_height(node) &&
+		(node.Index? ==> (forall child :: child in node.children ==> subtree_is_balanced(child))) &&
+		(node.Index? ==> (forall child :: child in node.children ==> max_height(child) == max_height(node.children[0])))
 }
 
-lemma children_have_lower_max_height(node: Node)
-	requires node.Index?;
-	ensures forall i :: 0 <= i < |node.children| ==> max_height(node.children[i]) == max_height(node) - 1;
+function method height(node: Node) : int
+	requires subtree_is_well_formed(node);
+	requires subtree_is_balanced(node);
+	ensures min_height(node) <= height(node) <= max_height(node);
 {
-	assume false;
-	if |node.children| > 0 {
-		assert max_height(node.children[0]) == max_height(node) - 1;
+	match node {
+		case Leaf(keys, values) => 0
+		case Index(pivots, children) =>
+			1 + height(children[0])
 	}
 }
 
-// predicate subtree_is_balanced(node: Node)
-// 	requires subtree_is_well_formed(node);
-// {
-// 	min_height(node) == max_height(node)
-// }
+lemma children_have_one_less_height(node: Node)
+	requires subtree_is_well_formed(node);
+	requires subtree_is_balanced(node);
+	ensures node.Index? ==> forall child :: child in node.children ==> height(child) == height(node) - 1;
+{
+	if node.Index? {
+		assert forall child :: child in node.children ==> height(child) == height(node) - 1;
+	}
+}
 
-// datatype Config = Config(
-// 	min_leaf_size: int, max_leaf_size: int,
-//   min_fanout: int, max_fanout: int)
+predicate is_child_list(nodes: seq<Node>)
+{
+	|nodes| > 0 &&
+		(forall node :: node in nodes ==> subtree_is_well_formed(node)) &&
+		(forall node :: node in nodes ==> subtree_is_balanced(node)) &&
+		(forall node :: node in nodes ==> height(node) == height(nodes[0]))
+}
 
-// predicate well_formed_config(cfg: Config) {
-// 	1 <= cfg.min_leaf_size < cfg.max_leaf_size &&
-// 	2 <= cfg.min_fanout < cfg.max_fanout
-// }
+function method set_of_keys_of_children(nodes: seq<Node>) : set<string>
+	requires is_child_list(nodes);
+{
+	if |nodes| == 1 then set_of_keys(nodes[0])
+	else set_of_keys(nodes[0]) + set_of_keys_of_children(nodes[1..])
+}
 
-// predicate subtree_satisfies_config(node: Node, cfg: Config) {
-// 	match node {
-// 		case Leaf(keys, pivots) =>
-// 			cfg.min_leaf_size <= |keys| <= cfg.max_leaf_size
-// 		case Index(pivots, children) =>
-// 			cfg.min_fanout <= |children| < cfg.max_fanout &&
-// 			forall i :: 0 <= i < |children| ==> subtree_satisfies_config(children[i], cfg)
-// 	}
-// }
+function method set_of_keys(node: Node) : set<string>
+	requires subtree_is_well_formed(node);
+	requires subtree_is_balanced(node);
+{	
+	match node {
+		case Leaf(keys, values) =>
+			set k | k in multiset(keys)
+		case Index(pivots, children) =>
+			children_have_one_less_height(node);
+			set_of_keys_of_children(children)
+	}
+}
 
-// predicate is_valid_b_subtree(node: Node, cfg: Config) {
-// 	subtree_is_well_formed(node) &&
-// 		subtree_is_sorted(node) &&
-// 		subtree_is_balanced(node) &&
-// 		subtree_satisfies_config(node, cfg)
-// }
+predicate seq_is_strictly_increasing(ss: seq<string>) {
+	forall i :: 0 <= i < |ss|-1 ==> lexical_cmp(ss[i], ss[i+1]) < 0
+}		
 
-// datatype QueryResult = KeyDoesNotExist | Value(v: int)
+predicate subtree_is_sorted(node: Node)
+	requires subtree_is_well_formed(node);
+	requires subtree_is_balanced(node);
+{
+	match node {
+		case Leaf(keys, values) =>
+			seq_is_strictly_increasing(keys)
+		case Index(pivots, children) =>
+			seq_is_strictly_increasing(pivots) &&
+			(forall i :: 0 <= i < |children|-1 ==>
+			  (forall x :: x in set_of_keys(children[i]) ==>
+			    lexical_cmp(x, pivots[i]) < 0)) &&
+			(forall i :: 1 <= i < |children| ==>
+			  (forall x :: x in set_of_keys(children[i]) ==>
+			    lexical_cmp(pivots[i-1], x) <= 0)) &&
+			forall i :: 0 <= i < |children| ==> subtree_is_sorted(children[i])
+	}
+}
 
-// function method search_seq(keys: seq<string>, values: seq<int>, key: string) : QueryResult
-// 	requires seq_is_strictly_increasing(keys);
-// 	requires |keys| == |values|;
-// 	ensures key !in map_of_kvpairs(map[], keys, values) ==>
-// 		search_seq(keys, values, key) == KeyDoesNotExist;
-// 	ensures key in map_of_kvpairs(map[], keys, values) ==>
-// 		search_seq(keys, values, key) == Value(map_of_kvpairs(map[], keys, values)[key]);
-// {
-// 	if |keys| == 0 then KeyDoesNotExist
-// 	else if keys[0] == key then Value(values[0])
-// 	else search_seq(keys[1..], values[1..], key)
-// }
-	
-// // function method query(node: Node, key: string) : QueryResult
-// // 	requires subtree_is_well_formed(node);
-// // 	requires subtree_is_sorted(node);
-// // 	ensures key !in subtree_map_contents(node) <==> query(node, key) == KeyDoesNotExist;
-// // 	ensures key in subtree_map_contents(node) <==> query(node, key) == Value(subtree_map_contents(node)[key]);
-// // {
+function map_of_kvpairs(acc: map<string, int>, keys: seq<string>, values: seq<int>) : map<string, int>
+	requires |keys| == |values|;
+{
+	if |keys| == 0 then acc
+	else map_of_kvpairs(acc, keys[1..], values[1..])[keys[0] := values[0]]
+}
+
+function map_of_children(acc: map<string, int>, nodes: seq<Node>) : map<string, int>
+	requires is_child_list(nodes);
+	requires forall child :: child in nodes ==> subtree_is_sorted(child);
+	decreases height(nodes[0]), |nodes|, 1;
+{
+	if |nodes| == 1 then map_of_subtree(acc, nodes[0])
+	else map_of_children(map_of_subtree(acc, nodes[0]), nodes[1..])
+}
+
+function map_of_subtree(acc: map<string, int>, node: Node) : map<string, int>
+	requires subtree_is_well_formed(node);
+	requires subtree_is_balanced(node);
+	requires subtree_is_sorted(node);
+	decreases height(node), 0;
+{
+	match node {
+		case Leaf(keys, values) =>
+			map_of_kvpairs(acc, keys, values)
+		case Index(pivots, children) =>
+			children_have_one_less_height(node);
+			map_of_children(acc, children)
+	}
+}
+
+function subtree_map_contents(node: Node) : map<string, int>
+	requires subtree_is_well_formed(node);
+	requires subtree_is_balanced(node);
+	requires subtree_is_sorted(node);
+{
+	map_of_subtree(map[], node)
+}
+
+// // datatype Config = Config(
+// // 	min_leaf_size: int, max_leaf_size: int,
+// //   min_fanout: int, max_fanout: int)
+
+// // predicate well_formed_config(cfg: Config) {
+// // 	1 <= cfg.min_leaf_size < cfg.max_leaf_size &&
+// // 	2 <= cfg.min_fanout < cfg.max_fanout
+// // }
+
+// // predicate subtree_satisfies_config(node: Node, cfg: Config) {
 // // 	match node {
-// // 		case Leaf(keys, values) =>
-			
+// // 		case Leaf(keys, pivots) =>
+// // 			cfg.min_leaf_size <= |keys| <= cfg.max_leaf_size
 // // 		case Index(pivots, children) =>
+// // 			cfg.min_fanout <= |children| < cfg.max_fanout &&
+// // 			forall i :: 0 <= i < |children| ==> subtree_satisfies_config(children[i], cfg)
 // // 	}
 // // }
+
+// // predicate is_valid_b_subtree(node: Node, cfg: Config) {
+// // 	subtree_is_well_formed(node) &&
+// // 		subtree_is_sorted(node) &&
+// // 		subtree_is_balanced(node) &&
+// // 		subtree_satisfies_config(node, cfg)
+// // }
+
+// // datatype QueryResult = KeyDoesNotExist | Value(v: int)
+
+// // function method search_seq(keys: seq<string>, values: seq<int>, key: string) : QueryResult
+// // 	requires seq_is_strictly_increasing(keys);
+// // 	requires |keys| == |values|;
+// // 	ensures key !in map_of_kvpairs(map[], keys, values) ==>
+// // 		search_seq(keys, values, key) == KeyDoesNotExist;
+// // 	ensures key in map_of_kvpairs(map[], keys, values) ==>
+// // 		search_seq(keys, values, key) == Value(map_of_kvpairs(map[], keys, values)[key]);
+// // {
+// // 	if |keys| == 0 then KeyDoesNotExist
+// // 	else if keys[0] == key then Value(values[0])
+// // 	else search_seq(keys[1..], values[1..], key)
+// // }
+	
+// // // function method query(node: Node, key: string) : QueryResult
+// // // 	requires subtree_is_well_formed(node);
+// // // 	requires subtree_is_sorted(node);
+// // // 	ensures key !in subtree_map_contents(node) <==> query(node, key) == KeyDoesNotExist;
+// // // 	ensures key in subtree_map_contents(node) <==> query(node, key) == Value(subtree_map_contents(node)[key]);
+// // // {
+// // // 	match node {
+// // // 		case Leaf(keys, values) =>
+			
+// // // 		case Index(pivots, children) =>
+// // // 	}
+// // // }
